Strata/Languages/Core/StatementSemantics.lean
@@ -56,6 +56,7 @@ instance : HasBool Core.Expression where
   tt := Core.true
   ff := Core.false
   tt_is_not_ff := by unfold Core.true Core.false; unfold Lambda.LExpr.boolConst; simp
+  boolTy := .forAll [] (.tcons "bool" [])
 
 instance : HasNot Core.Expression where
   not
