StrataTest/DL/Imperative/DDMTranslate.lean
@@ -50,7 +50,7 @@ instance : ToFormat TransBindings where
                  varGen: {b.varGen}"
 
 instance : Inhabited (TransBindings × Arith.Command) where
-  default := ({}, .havoc "default_var" .empty)
+  default := ({}, .set "default_var" .nondet .empty)
 
 /--
 info: inductive ArithPrograms.ArithProgramsType : Type → Type
@@ -139,7 +139,7 @@ ArithPrograms.Command.havoc : {α : Type} → α → Strata.Ann String α → Co
 #print Command
 
 instance : Inhabited (Arith.Command × TransBindings) where
-  default := (.havoc "default" .empty, {})
+  default := (.set "default" .nondet .empty, {})
 
 instance : Inhabited (Arith.Commands × TransBindings) where
   default := ([], {})
@@ -151,15 +151,15 @@ def translateCommand (bindings : TransBindings) (c : ArithPrograms.Command α) :
     let bindings := { bindings with freeVars := bindings.freeVars ++ [name.val] }
     let tp := translateType tp
     let (init_var_name, bindings) := genInitVar bindings name.val
-    return ((.init name.val tp (some (.Var init_var_name tp)) .empty), bindings)
+    return ((.init name.val tp (.det (.Var init_var_name tp)) .empty), bindings)
   | .init _ name tp expr =>
     let tp := translateType tp
     let expr ← translateExpr bindings expr
     let bindings := { bindings with freeVars := bindings.freeVars ++ [name.val] }
-    return ((.init name.val tp (some expr) .empty), bindings)
+    return ((.init name.val tp (.det expr) .empty), bindings)
   | .assign _ label expr =>
     let expr ← translateExpr bindings expr
-    return ((.set label.val expr .empty), bindings)
+    return ((.set label.val (.det expr) .empty), bindings)
   | .assume _ label expr =>
     let label ← translateLabel bindings label
     let expr ← translateExpr bindings expr
@@ -169,7 +169,7 @@ def translateCommand (bindings : TransBindings) (c : ArithPrograms.Command α) :
     let expr ← translateExpr bindings expr
     return ((.assert label expr .empty), bindings)
   | .havoc _ name =>
-    return ((.havoc name.val .empty), bindings)
+    return ((.set name.val .nondet .empty), bindings)
 
 partial def translateProgram (ops : Array Strata.Operation) : TransM Arith.Commands := do
   let (cmds, _) ← go 0 ops.size {} ops
